error example for exact? : "found a proof, but the corresponding tactic failed:"

LeanStudy/QuickSort.lean
@@ -1,9 +1,59 @@
 import Lean
 import Mathlib.Tactic.Ring
+import Mathlib.Data.List.Basic
 
-theorem filter_length : ∀ {α : Type} (p : α → Prop) [DecidablePred p] (xs : List α),
+def my_partition {α : Type} (p : α → Bool) (as : List α) : List α × List α :=
+  loop p as ([], [])
+where
+  @[specialize] loop (p : α → Bool): List α → List α × List α → List α × List α
+  | [],    (bs, cs) => (bs.reverse, cs.reverse)
+  | a::as, (bs, cs) =>
+    match p a with
+    | true  => loop p as (a::bs, cs)
+    | false => loop p as (bs, a::cs)
+
+lemma partition_loop_length {α : Type} (p : α → Bool) (as : List α) (bs cs : List α) :
+  (my_partition.loop p as (bs, cs)).1.length + (my_partition.loop p as (bs, cs)).2.length = as.length + bs.length + cs.length := by
+  induction as generalizing bs cs with
+  | nil =>
+    rw [my_partition.loop]
+    simp
+  | cons a as ih =>
+    simp only [my_partition.loop]
+    by_cases hpa : p a
+    .
+      simp only [hpa, decide_true]
+      simp only [ih]
+      simp only [List.length_cons]
+      ring
+    .
+      simp only [hpa, decide_false]
+      simp only [ih]
+      simp only [List.length_cons]
+      ring
+
+lemma partition_length {α : Type} (p : α → Bool) (as : List α) :
+  (my_partition p as).1.length + (my_partition p as).2.length = as.length := by
+  induction as with
+  | nil => rfl
+  | cons a as ih =>
+    simp only [my_partition]
+    by_cases hpa : p a
+    .
+      simp only [my_partition.loop]
+      simp only [hpa, decide_true]
+      simp only [List.length_cons]
+      rw [partition_loop_length]
+      simp only [List.length_cons, List.length_nil, zero_add, add_zero]
+    .
+      simp only [my_partition.loop]
+      simp only [hpa, decide_false]
+      simp only [List.length_cons]
+      rw [partition_loop_length]
+      simp only [List.length_cons, List.length_nil, zero_add, add_zero]
+
+theorem filter_length {α : Type} (p : α → Prop) [DecidablePred p] (xs : List α) :
   (xs.filter p).length ≤ xs.length := by
-    intros α p h xs
     induction xs with
     | nil => rfl
     | cons x xs ih =>
@@ -16,7 +66,7 @@ theorem filter_length : ∀ {α : Type} (p : α → Prop) [DecidablePred p] (xs 
         simp only [hpx, decide_false]
         calc
           _ ≤ xs.length := by simp only [ih]
-          _ ≤ xs.length + 1 := by apply Nat.le_add_right
+          _ ≤ xs.length + 1 := by exact Nat.le_add_right xs.length 1
 
 def my_quick_sort {α : Type} [LT α][DecidableLT α] : List α → List α :=
   λ l => match hl : l with
@@ -29,6 +79,14 @@ def my_quick_sort {α : Type} [LT α][DecidableLT α] : List α → List α :=
     let larger := parted.2
     have p_decidable : DecidablePred p := by
       infer_instance
+    have list_filter_lemma :
+      (List.filter (fun b ↦ decide (b < pivot)) xs).length < xs.length + 1 := by
+      calc
+        _ ≤ xs.length := by apply filter_length
+        _ < xs.length + 1 := by exact lt_add_one xs.length
+    have filter_length_lemma (xs : List α):
+      (xs.filter p).length ≤ xs.length := by
+      apply filter_length
     have : smaller.length < l.length := by
       simp only [parted, larger, smaller]
       simp only [List.partition_eq_filter_filter]
@@ -36,7 +94,7 @@ def my_quick_sort {α : Type} [LT α][DecidableLT α] : List α → List α :=
       rw [List.length_cons]
       calc
         _ ≤ xs.length := by
-          sorry
+          exact?
         _ < xs.length + 1 := by
           exact lt_add_one xs.length
     have : larger.length < l.length := by
@@ -46,12 +104,8 @@ def my_quick_sort {α : Type} [LT α][DecidableLT α] : List α → List α :=
       rw [List.length_cons]
       calc
         _ ≤ xs.length := by
-          sorry
+          exact?
         _ < xs.length + 1 := by
           exact lt_add_one xs.length
-    have : (List.filter (fun b ↦ decide (b < pivot)) xs).length < xs.length + 1 := by
-      calc
-        _ ≤ xs.length := by apply filter_length
-        _ < xs.length + 1 := by exact lt_add_one xs.length
     my_quick_sort smaller ++ [pivot] ++ my_quick_sort larger
 termination_by x1 => x1.length
